Tests/Aiur.lean
@@ -4,3 +4,4 @@ public import Tests.Aiur.Common
 public import Tests.Aiur.Aiur
 public import Tests.Aiur.Hashes
 public import Tests.Aiur.RBTreeMap
+public import Tests.Aiur.Cross
